stateful spec

specs/Spec.Chacha20.ST.fst
@@ -7,111 +7,15 @@ module ST = FStar.HyperStack.ST
 //open FStar.Mul
 open FStar.Seq
 open FStar.UInt32
-open FStar.Endianness
 open Spec.Lib
-open Spec.Chacha20.Lemmas
-open Seq.Create
-
-
-(* Generic key-value state monad: WIP *)
-noeq 
-type kv (a:Type) = 
-  |  MkSt: k: Type -> v: Type -> 
-	   get:(a -> k -> Tot v) -> 
-	   set:(a -> k -> v -> Tot a) -> kv a
-
-     
-type stateful (a:Type) (b:Type) =
-	      a -> Tot (b * a)
-
-val stateful_read: #a:Type -> kv:kv a -> key:kv.k -> Tot (stateful a kv.v)	   
-let stateful_read  #a kv key = 
-    fun m -> kv.get m key, m
-
-val stateful_write: #a:Type -> kv:kv a -> key:kv.k -> value:kv.v -> Tot (stateful a unit)	   
-let stateful_write  #a kv key value = 
-    fun m -> (), kv.set m key value
-
-val stateful_return: #a: Type -> #b:Type -> r:b -> Tot (stateful a b)
-let stateful_return #a #b r = 
-    fun m -> r, m
-    
-val stateful_bind: #a:Type -> #b:Type -> #c:Type -> stateful a b -> (b -> Tot (stateful a c)) -> Tot (stateful a c)
-let stateful_bind #a #b #c f g = fun s -> let (a,s) = f s in g a s
-
-type u32 = FStar.UInt32.t
-
-// state monad for manipulating one sequence
-type seq_l 'a n = m: seq 'a{length m = n}
-type index_l n = m: nat{m < n}
-type seq1_st s n b =
-     seq_l s n -> Tot (b * seq_l s n)
-
-val seq1_read: #a:Type -> #n:nat -> (i:index_l n) -> Tot (seq1_st a n a)
-let seq1_read  #a #n i = fun m -> Seq.index m i, m
-
-val seq1_copy: #a:Type -> #n:nat -> Tot (seq1_st a n (seq_l a n))
-let seq1_copy  #a #n = fun m -> m, m
-
-
-val seq1_return: #a:Type -> #n:nat -> #b:Type -> x:b -> seq1_st a n b
-let seq1_return #a #n #b w = fun m -> (w,m)
-
-val seq1_write: #a:Type -> #n:nat -> (i:index_l n) -> (v:a) -> Tot (seq1_st a n unit)
-let seq1_write #a #n i x = fun m ->  (), (m.[i] <- x)
-
-val seq1_bind: #a:Type -> #n:nat -> #b:Type -> #c:Type -> seq1_st a n b -> (b -> seq1_st a n c) -> Tot (seq1_st a n c)
-let seq1_bind #a #n #b #c f g = fun s -> let a, s = f s in g a s
-
-val seq1_iter: #a:Type -> #n:nat -> c:nat -> seq1_st a n unit -> Tot (seq1_st a n unit)
-let seq1_iter #a #m n f = 
-    let f' (s:seq_l a m) : Tot (seq_l a m) = 
-        let s' = f s in
-	snd s'
-    in
-    fun s -> (),iter 10 f' s
-
-val seq1_in_place_map2: #a:Type -> #n:nat -> #b:Type -> f:(a -> b -> Tot a) -> s:seq_l b n -> Tot (seq1_st a n unit)
-let seq1_in_place_map2  #a #m #b f i = 
-    fun s -> 
-      let s' = Spec.Loops.seq_map2 f s i in
-      (),s'
-
-val seq1_alloc: #a:Type -> #n:nat -> #b:Type -> init:a -> f:seq1_st a n b -> Tot b
-let seq1_alloc #a #n #b init f =
-    let s = Seq.create n init in
-    let s' = f s in
-    fst s'
-
-val seq1_uint32s_from_le: #n:nat -> b:bytes -> start:nat -> len: nat{
-						     length b = FStar.Mul.(4 * len)
-					 	   /\ start + len <= n} -> 
-		     Tot (seq1_st u32 n unit) 
-let seq1_uint32s_from_le #n src start len =
-  fun s ->
-    let s' = uint32s_from_le len src in
-    let s0,s_ = split s start in
-    let s1,s2 = split s_ len in
-    (), s0 @| s' @| s2
-
-val seq1_uint32s_to_le: #n:nat -> start:nat -> len: nat{start + len <= n} -> 
-		     Tot (seq1_st u32 n (lbytes (FStar.Mul.(4 * len)))) 
-let seq1_uint32s_to_le #n start len =
-  fun s ->
-    if len = 0 then
-       Seq.createEmpty, s
-    else
-       let s0,s_ = split s start in
-       let s1,s2 = split s_ len in
-       let b = uint32s_to_le len s1 in
-       b, s
-
 
 (* Chacha20 State *)
 // internally, blocks are represented as 16 x 4-byte integers
 type chacha_st 'b = seq1_st u32 16 'b
 type st = seq_l u32 16
 let idx = index_l 16
+
+(* Wrapper monadic functions specialized for the Chacha state *)
 let copy : chacha_st st = seq1_copy #u32 #16 
 let read i : chacha_st u32 = seq1_read #u32 #16 i
 let write i x : chacha_st unit = seq1_write #u32 #16 i x
@@ -120,16 +24,16 @@ let bind (f:chacha_st 'b) (g:'b -> chacha_st 'c) : chacha_st 'c = seq1_bind f g
 let iter (n:nat) (f:chacha_st unit) = seq1_iter n f
 let in_place_map2 (f:u32 -> u32 -> Tot u32) (s:st) = seq1_in_place_map2 f s
 let alloc (f:chacha_st 'b) = seq1_alloc 0ul f
-let uint32s_from_le src (start:idx) 
-		    (len:nat{FStar.Mul.(len * 4 = length src)
-			   /\ start + len <= 16}): chacha_st unit = 
-		seq1_uint32s_from_le src start len
-let uint32s_to_le (start:idx) 
-		  (len:nat{start + len <= 16}): chacha_st (lbytes FStar.Mul.(4 * len)) = 
-		seq1_uint32s_to_le start len
+let uint32s_from_le src (start:idx) (len:nat{FStar.Mul.(len * 4 = length src)
+					    /\ start + len <= 16}): chacha_st unit = 
+	seq1_uint32s_from_le src start len
+let uint32s_to_le (start:idx) (len:nat{start + len <= 16})
+		  : chacha_st (lbytes FStar.Mul.(4 * len)) = 
+	seq1_uint32s_to_le start len
 
 
-(* Chacha20 Code *)
+(* Chacha20 Spec *)
+
 let keylen = 32   (* in bytes *)
 let blocklen = 64 (* in bytes *)
 let noncelen = 12 (* in bytes *)
@@ -193,8 +97,6 @@ let setup (k:key) (n:nonce) (c:counter): chacha_st unit =
   write 12 (UInt32.uint_to_t c) ;;
   uint32s_from_le n 13 3
 
-
-
 let chacha20_block (k:key) (n:nonce) (c:counter): Tot block =
     alloc (
        setup k n c ;;
@@ -212,10 +114,11 @@ let chacha20_ctx: Spec.CTR.block_cipher_ctx =
     incr = 1
     }
 
-let chacha20_cipher: Spec.CTR.block_cipher chacha20_ctx = chacha20_block
+let chacha20_block_cipher: Spec.CTR.block_cipher chacha20_ctx = chacha20_block
 
 let chacha20_encrypt_bytes key nonce counter m =
-    Spec.CTR.counter_mode chacha20_ctx chacha20_cipher key nonce counter m
+    let chacha20_ctr = Spec.CTR.counter_mode chacha20_ctx chacha20_block_cipher in
+    chacha20_ctr key nonce counter m
 
 
 unfold let test_plaintext = [
@@ -266,6 +169,7 @@ unfold let test_nonce = [
 
 unfold let test_counter = 1
 
+open Seq.Create
 let test() =
   assert_norm(List.Tot.length test_plaintext = 114);
   assert_norm(List.Tot.length test_ciphertext = 114);
