specs/Spec.Lib.fst
@@ -2,10 +2,11 @@ module Spec.Lib
 
 module ST = FStar.HyperStack.ST
 
-open FStar.Mul
 open FStar.Seq
 open FStar.UInt32
 open FStar.Endianness
+
+let op_Star_Star = FStar.Mul.op_Star
 
 #set-options "--initial_fuel 0 --initial_ifuel 0 --max_fuel 0 --max_ifuel 0"
 
@@ -103,24 +104,15 @@ let lemma_uint32_from_to_bij (b:lbytes 4) : Lemma
     if uint32_to_le (uint32_from_le b) <> b then lemma (uint32_to_le (uint32_from_le b)) b
 
 
-val uint32s_from_le: len:nat -> b:lbytes (4 * len) -> Tot (s:seq UInt32.t{length s = len}) (decreases len)
+val uint32s_from_le: len:nat -> b:lbytes (4 ** len) -> Tot (s:seq UInt32.t{length s = len}) (decreases len)
 let rec uint32s_from_le len src =
   if len = 0 then createEmpty
   else (
-    let prefix, last = split src (4 * len - 4) in
+    let prefix, last = split src (4 ** len - 4) in
     snoc (uint32s_from_le (len-1) prefix) (uint32_from_le last)
   )
 
-    (* uint32s_from_le (len - 1)  *)
-(* let rec uint32s_from_le len src = *)
-(*   if len = 0 then Seq.createEmpty #UInt32.t *)
-(*   else *)
-(*     let h = slice src 0 4 in *)
-(*     let t = slice src 4 (4*len) in *)
-(*     Seq.cons (uint32_from_le h) *)
-(*              (uint32s_from_le (len-1) t) *)
-
-val uint32s_to_le: len:nat -> s:seq UInt32.t{length s = len} -> Tot (lbytes (4 * len))  (decreases len)
+val uint32s_to_le: len:nat -> s:seq UInt32.t{length s = len} -> Tot (lbytes (4 ** len))  (decreases len)
 let rec uint32s_to_le len src =
   if len = 0 then createEmpty
   else (
@@ -129,15 +121,15 @@ let rec uint32s_to_le len src =
     uint32s_to_le (len-1) prefix @| (uint32_to_le last)
   )
 
-val uint64s_from_le: len:nat -> b:lbytes (8 * len) -> Tot (s:seq UInt64.t{length s = len}) (decreases len)
+val uint64s_from_le: len:nat -> b:lbytes (8 ** len) -> Tot (s:seq UInt64.t{length s = len}) (decreases len)
 let rec uint64s_from_le len src =
   if len = 0 then createEmpty
   else (
-    let prefix, last = split src (8 * len - 8) in
+    let prefix, last = split src (8 ** len - 8) in
     snoc (uint64s_from_le (len-1) prefix) (uint64_from_le last)
   )
 
-val uint64s_to_le: len:nat -> s:seq UInt64.t{length s = len} -> Tot (lbytes (8 * len))  (decreases len)
+val uint64s_to_le: len:nat -> s:seq UInt64.t{length s = len} -> Tot (lbytes (8 ** len))  (decreases len)
 let rec uint64s_to_le len src =
   if len = 0 then createEmpty
   else (
@@ -147,15 +139,15 @@ let rec uint64s_to_le len src =
   )
 
 
-val uint32s_from_be: len:nat -> b:lbytes (4 * len) -> Tot (s:seq UInt32.t{length s = len}) (decreases len)
+val uint32s_from_be: len:nat -> b:lbytes (4 ** len) -> Tot (s:seq UInt32.t{length s = len}) (decreases len)
 let rec uint32s_from_be len src =
   if len = 0 then createEmpty
   else (
-    let prefix, last = split src (4 * len - 4) in
+    let prefix, last = split src (4 ** len - 4) in
     snoc (uint32s_from_be (len-1) prefix) (uint32_from_be last)
   )
 
-val uint32s_to_be: len:nat -> s:seq UInt32.t{length s = len} -> Tot (lbytes (4 * len))  (decreases len)
+val uint32s_to_be: len:nat -> s:seq UInt32.t{length s = len} -> Tot (lbytes (4 ** len))  (decreases len)
 let rec uint32s_to_be len src =
   if len = 0 then createEmpty
   else (
@@ -164,15 +156,15 @@ let rec uint32s_to_be len src =
     uint32s_to_be (len-1) prefix @| (uint32_to_be last)
   )
 
-val uint64s_from_be: len:nat -> b:lbytes (8 * len) -> Tot (s:seq UInt64.t{length s = len}) (decreases len)
+val uint64s_from_be: len:nat -> b:lbytes (8 ** len) -> Tot (s:seq UInt64.t{length s = len}) (decreases len)
 let rec uint64s_from_be len src =
   if len = 0 then createEmpty
   else (
-    let prefix, last = split src (8 * len - 8) in
+    let prefix, last = split src (8 ** len - 8) in
     snoc (uint64s_from_be (len-1) prefix) (uint64_from_be last)
   )
 
-val uint64s_to_be: len:nat -> s:seq UInt64.t{length s = len} -> Tot (lbytes (8 * len))  (decreases len)
+val uint64s_to_be: len:nat -> s:seq UInt64.t{length s = len} -> Tot (lbytes (8 ** len))  (decreases len)
 let rec uint64s_to_be len src =
   if len = 0 then createEmpty
   else (
@@ -184,12 +176,12 @@ let rec uint64s_to_be len src =
 
 #reset-options "--initial_fuel 1 --max_fuel 1 --z3rlimit 20"
 
-let lemma_uint32s_from_le_def_0 (len:nat{len = 0}) (b:lbytes (4*len)) : Lemma
+let lemma_uint32s_from_le_def_0 (len:nat{len = 0}) (b:lbytes (4**len)) : Lemma
   (uint32s_from_le len b == Seq.createEmpty)
   = ()
-let lemma_uint32s_from_le_def_1 (len:nat{len > 0}) (b:lbytes (4*len)) : Lemma
-  (uint32s_from_le len b == Seq.snoc (uint32s_from_le (len-1) (slice b 0 (4*len - 4)))
-                                     (uint32_from_le (slice b (4*len - 4) (4*len)))
+let lemma_uint32s_from_le_def_1 (len:nat{len > 0}) (b:lbytes (4**len)) : Lemma
+  (uint32s_from_le len b == Seq.snoc (uint32s_from_le (len-1) (slice b 0 (4**len - 4)))
+                                     (uint32_from_le (slice b (4**len - 4) (4**len)))
   )
   = ()
 
@@ -203,12 +195,12 @@ let lemma_uint32s_to_le_def_1 (len:nat{len > 0}) (s:seq UInt32.t{length s = len}
   = ()
 
 
-let lemma_uint32s_from_be_def_0 (len:nat{len = 0}) (b:lbytes (4*len)) : Lemma
+let lemma_uint32s_from_be_def_0 (len:nat{len = 0}) (b:lbytes (4**len)) : Lemma
   (uint32s_from_be len b == Seq.createEmpty)
   = ()
-let lemma_uint32s_from_be_def_1 (len:nat{len > 0}) (b:lbytes (4*len)) : Lemma
-  (uint32s_from_be len b == Seq.snoc (uint32s_from_be (len-1) (slice b 0 (4*len - 4)))
-                                     (uint32_from_be (slice b (4*len - 4) (4*len)))
+let lemma_uint32s_from_be_def_1 (len:nat{len > 0}) (b:lbytes (4**len)) : Lemma
+  (uint32s_from_be len b == Seq.snoc (uint32s_from_be (len-1) (slice b 0 (4**len - 4)))
+                                     (uint32_from_be (slice b (4**len - 4) (4**len)))
   )
   = ()
 
@@ -222,12 +214,12 @@ let lemma_uint32s_to_be_def_1 (len:nat{len > 0}) (s:seq UInt32.t{length s = len}
   = ()
 
 
-let lemma_uint64s_from_be_def_0 (len:nat{len = 0}) (b:lbytes (8*len)) : Lemma
+let lemma_uint64s_from_be_def_0 (len:nat{len = 0}) (b:lbytes (8**len)) : Lemma
   (uint64s_from_be len b == Seq.createEmpty)
   = ()
-let lemma_uint64s_from_be_def_1 (len:nat{len > 0}) (b:lbytes (8*len)) : Lemma
-  (uint64s_from_be len b == Seq.snoc (uint64s_from_be (len-1) (slice b 0 (8*len - 8)))
-                                     (uint64_from_be (slice b (8*len - 8) (8*len)))
+let lemma_uint64s_from_be_def_1 (len:nat{len > 0}) (b:lbytes (8**len)) : Lemma
+  (uint64s_from_be len b == Seq.snoc (uint64s_from_be (len-1) (slice b 0 (8**len - 8)))
+                                     (uint64_from_be (slice b (8**len - 8) (8**len)))
   )
   = ()
 
@@ -243,16 +235,16 @@ let lemma_uint64s_to_be_def_1 (len:nat{len > 0}) (s:seq UInt64.t{length s = len}
 
 #reset-options "--initial_fuel 0 --max_fuel 0 --z3rlimit 20"
 
-let rec lemma_uint32s_from_le_inj (len:nat) (b:lbytes (4 * len)) (b':lbytes (4 * len)) : Lemma
+let rec lemma_uint32s_from_le_inj (len:nat) (b:lbytes (4 ** len)) (b':lbytes (4 ** len)) : Lemma
   (requires (uint32s_from_le len b == uint32s_from_le len b'))
   (ensures  (b == b'))
   = if len = 0 then (lemma_uint32s_from_le_def_0 len b; lemma_uint32s_from_le_def_0 len b';
       Seq.lemma_eq_intro b b')
     else (
-          let h  = slice b (4*len - 4) (4*len) in
-          let h'  = slice b' (4*len - 4) (4*len) in
-          let t  = slice b 0 (4*len-4) in
-          let t' = slice b' 0 (4*len-4) in
+          let h  = slice b (4**len - 4) (4**len) in
+          let h'  = slice b' (4**len - 4) (4**len) in
+          let t  = slice b 0 (4**len-4) in
+          let t' = slice b' 0 (4**len-4) in
           lemma_uint32s_from_le_def_1 len b;
           lemma_uint32s_from_le_def_1 len b';
           Seq.lemma_eq_intro (uint32s_from_le len b) (uint32s_from_le len b');
@@ -273,7 +265,7 @@ let rec lemma_uint32s_from_le_inj (len:nat) (b:lbytes (4 * len)) (b':lbytes (4 *
 
 #set-options "--max_fuel 0 --z3rlimit 100"
 
-let rec lemma_uint32s_from_le_bij (len:nat) (b:lbytes (4 * len)) : Lemma
+let rec lemma_uint32s_from_le_bij (len:nat) (b:lbytes (4 ** len)) : Lemma
   (requires (True))
   (ensures  (uint32s_to_le len (uint32s_from_le len b) == b))
   = if len = 0 then (
@@ -284,7 +276,7 @@ let rec lemma_uint32s_from_le_bij (len:nat) (b:lbytes (4 * len)) : Lemma
       lemma_uint32s_from_le_def_1 len b;
       let b' = uint32s_from_le len b in
       lemma_uint32s_to_le_def_1 len b';
-      lemma_uint32_from_to_bij (slice b (4*len-4) (length b));
+      lemma_uint32_from_to_bij (slice b (4**len-4) (length b));
       lemma_uint32s_from_le_bij (len - 1) (slice b 0 (length b - 4));
       lemma_eq_intro b'  (snoc (uint32s_from_le (len-1) (slice b 0 (length b - 4))) (uint32_from_le (slice b (length b - 4) (length b))));
       lemma_eq_intro (slice b' 0 (length b'-1)) (uint32s_from_le (len-1) (slice b 0 (length b - 4)));
@@ -308,13 +300,13 @@ let rec lemma_uint32s_to_le_inj (len:nat) (b:seq UInt32.t{length b = len})
       lemma_uint32s_to_le_def_1 len b;
       lemma_uint32s_to_le_def_1 len b';
       Seq.lemma_eq_intro (uint32s_to_le len b) (uint32s_to_le len b');
-      cut (Seq.slice (uint32s_to_le len b) (4*len-4) (4 * len) == Seq.slice (uint32s_to_le len b') (4*len -4) (4 * len));
-      Seq.lemma_eq_intro (Seq.slice (uint32s_to_le len b) (4*len-4) (4 * len)) (uint32_to_le h);
-      Seq.lemma_eq_intro (Seq.slice (uint32s_to_le len b') (4*len-4) (4 * len)) (uint32_to_le h');
+      cut (Seq.slice (uint32s_to_le len b) (4**len-4) (4 ** len) == Seq.slice (uint32s_to_le len b') (4**len -4) (4 ** len));
+      Seq.lemma_eq_intro (Seq.slice (uint32s_to_le len b) (4**len-4) (4 ** len)) (uint32_to_le h);
+      Seq.lemma_eq_intro (Seq.slice (uint32s_to_le len b') (4**len-4) (4 ** len)) (uint32_to_le h');
       lemma_uint32_to_le_inj h h';
-      cut (Seq.slice (uint32s_to_le len b) 0 (4*len-4) == Seq.slice (uint32s_to_le len b') 0 (4*len-4));
-      Seq.lemma_eq_intro (Seq.slice (uint32s_to_le len b) 0 (4*len-4)) (uint32s_to_le (len-1) t);
-      Seq.lemma_eq_intro (Seq.slice (uint32s_to_le len b') 0 (4*len-4)) (uint32s_to_le (len-1) t');
+      cut (Seq.slice (uint32s_to_le len b) 0 (4**len-4) == Seq.slice (uint32s_to_le len b') 0 (4**len-4));
+      Seq.lemma_eq_intro (Seq.slice (uint32s_to_le len b) 0 (4**len-4)) (uint32s_to_le (len-1) t);
+      Seq.lemma_eq_intro (Seq.slice (uint32s_to_le len b') 0 (4**len-4)) (uint32s_to_le (len-1) t');
       lemma_uint32s_to_le_inj (len-1) t t';
       Seq.lemma_eq_intro t t';
       Seq.lemma_eq_intro b (snoc t h);
@@ -337,7 +329,7 @@ let rec lemma_uint32s_to_le_bij (len:nat) (b:seq UInt32.t{length b = len}) : Lem
       lemma_uint32s_to_le_bij (len - 1) (slice b 0 (length b-1));
       lemma_eq_intro b' (append (uint32s_to_le (len-1) (slice b 0 (length b-1))) (uint32_to_le (index b (len-1))));
       lemma_eq_intro (slice b' 0 (length b' - 4)) (uint32s_to_le (len-1) (slice b 0 (length b-1)));
-      lemma_eq_intro (slice b' (4*len-4) (4*len)) (uint32_to_le (index b (len-1)));
+      lemma_eq_intro (slice b' (4**len-4) (4**len)) (uint32_to_le (index b (len-1)));
       lemma_eq_intro (uint32s_from_le len b') (snoc (uint32s_from_le (len-1) (uint32s_to_le (len-1) (slice b 0 (length b-1)))) (uint32_from_le (uint32_to_le (index b (len-1)))));
       lemma_eq_intro (uint32s_from_le len (uint32s_to_le len b)) b
     )
@@ -349,31 +341,31 @@ let lemma_append_assoc (#a:Type) (x:seq a) (y:seq a) (z:seq a) : Lemma
   (x @| (y @| z) == (x @| y) @| z) = lemma_eq_intro ((x @| y) @| z) (x @| (y @| z))
 
 
-val lemma_uint32s_from_le_slice: len:nat -> b:lbytes (4*len) -> n:nat{n <= len} -> Lemma
+val lemma_uint32s_from_le_slice: len:nat -> b:lbytes (4**len) -> n:nat{n <= len} -> Lemma
   (requires (True))
-  (ensures (uint32s_from_le len b == uint32s_from_le n (slice b 0 (4 * n)) @| uint32s_from_le (len - n) (slice b (4 * n) (length b))))
+  (ensures (uint32s_from_le len b == uint32s_from_le n (slice b 0 (4 ** n)) @| uint32s_from_le (len - n) (slice b (4 ** n) (length b))))
   (decreases (len-n))
 #reset-options "--initial_fuel 0 --max_fuel 0 --z3rlimit 50"
 let rec lemma_uint32s_from_le_slice len b n =
   if n = len then (
-    lemma_uint32s_from_le_def_0 0 (slice b (4*len) (4*len));
+    lemma_uint32s_from_le_def_0 0 (slice b (4**len) (4**len));
     lemma_eq_intro (slice b 0 (length b)) b;
-    lemma_eq_intro (uint32s_from_le 0 (slice b (4*len) (4*len))) createEmpty;
+    lemma_eq_intro (uint32s_from_le 0 (slice b (4**len) (4**len))) createEmpty;
     lemma_eq_intro (uint32s_from_le len b @| createEmpty) (uint32s_from_le len b)
   ) else (
     lemma_uint32s_from_le_def_1 len b;
-    lemma_uint32s_from_le_def_1 (len - n) (slice b (4 * n) (4 * len));
-    let tl, hd = split b (4*len - 4) in
+    lemma_uint32s_from_le_def_1 (len - n) (slice b (4 ** n) (4 ** len));
+    let tl, hd = split b (4**len - 4) in
     lemma_uint32s_from_le_slice (len-1) tl (n);
-    lemma_eq_intro (slice tl 0 (4*n)) (slice b 0 (4*n));
-    lemma_eq_intro (slice tl (4*n) (4*(len-1))) (slice b (4*n) (4 * (len - 1)));
-    lemma_append_assoc (uint32s_from_le n (slice tl 0 (4 * n)))
-                       (uint32s_from_le (len - 1 - n) (slice tl (4*n) (4*(len - 1))))
+    lemma_eq_intro (slice tl 0 (4**n)) (slice b 0 (4**n));
+    lemma_eq_intro (slice tl (4**n) (4**(len-1))) (slice b (4**n) (4 ** (len - 1)));
+    lemma_append_assoc (uint32s_from_le n (slice tl 0 (4 ** n)))
+                       (uint32s_from_le (len - 1 - n) (slice tl (4**n) (4**(len - 1))))
                        (create 1 (uint32_from_le hd));
-    lemma_eq_intro (slice b (4*len-4) (4*len)) (slice (slice b (4*n) (4*len)) (4*(len - 1 - n)) (4*(len-n)));
-    lemma_eq_intro (slice b (4*n) (4*(len-1))) (slice (slice b (4*n) (length b)) 0 (4 * (len - n - 1)));
+    lemma_eq_intro (slice b (4**len-4) (4**len)) (slice (slice b (4**n) (4**len)) (4**(len - 1 - n)) (4**(len-n)));
+    lemma_eq_intro (slice b (4**n) (4**(len-1))) (slice (slice b (4**n) (length b)) 0 (4 ** (len - n - 1)));
 
-    lemma_eq_intro (uint32s_from_le (len-n) (slice b (4 * n) (4*len))) (snoc (uint32s_from_le (len-n-1) (slice b (4*n) (4*(len-1)))) (uint32_from_le hd)))
+    lemma_eq_intro (uint32s_from_le (len-n) (slice b (4 ** n) (4**len))) (snoc (uint32s_from_le (len-n-1) (slice b (4**n) (4**(len-1)))) (uint32_from_le hd)))
 
 
 val lemma_uint32s_to_le_slice: len:nat -> b:Seq.seq UInt32.t{length b = len} -> n:nat{n <= len} -> Lemma
@@ -400,3 +392,97 @@ let rec lemma_uint32s_to_le_slice len b n =
     lemma_eq_intro (slice b n (len-1)) (slice (slice b n (len)) 0 (len-n-1));
     lemma_eq_intro (uint32s_to_le (len-n) (slice b n (len))) (uint32s_to_le (len-n-1) (slice b n (len-1)) @| uint32_to_le h)
   )
+
+(** Generic key-value state monad: WIP **)
+noeq 
+type kv (a:Type) = 
+  |  MkSt: k: Type -> v: Type -> 
+	   get:(a -> k -> Tot v) -> 
+	   set:(a -> k -> v -> Tot a) -> kv a
+
+     
+type stateful (a:Type) (b:Type) =
+	      a -> Tot (b * a)
+
+val stateful_read: #a:Type -> kv:kv a -> key:kv.k -> Tot (stateful a kv.v)	   
+let stateful_read  #a kv key = 
+    fun m -> kv.get m key, m
+
+val stateful_write: #a:Type -> kv:kv a -> key:kv.k -> value:kv.v -> Tot (stateful a unit)	   
+let stateful_write  #a kv key value = 
+    fun m -> (), kv.set m key value
+
+val stateful_return: #a: Type -> #b:Type -> r:b -> Tot (stateful a b)
+let stateful_return #a #b r = 
+    fun m -> r, m
+    
+val stateful_bind: #a:Type -> #b:Type -> #c:Type -> stateful a b -> (b -> Tot (stateful a c)) -> Tot (stateful a c)
+let stateful_bind #a #b #c f g = fun s -> let (a,s) = f s in g a s
+
+type u32 = FStar.UInt32.t
+
+// state monad for manipulating one sequence
+type seq_l 'a n = m: seq 'a{length m = n}
+type index_l n = m: nat{m < n}
+type seq1_st s n b =
+     seq_l s n -> Tot (b * seq_l s n)
+
+val seq1_read: #a:Type -> #n:nat -> (i:index_l n) -> Tot (seq1_st a n a)
+let seq1_read  #a #n i = fun m -> Seq.index m i, m
+
+val seq1_copy: #a:Type -> #n:nat -> Tot (seq1_st a n (seq_l a n))
+let seq1_copy  #a #n = fun m -> m, m
+
+
+val seq1_return: #a:Type -> #n:nat -> #b:Type -> x:b -> seq1_st a n b
+let seq1_return #a #n #b w = fun m -> (w,m)
+
+val seq1_write: #a:Type -> #n:nat -> (i:index_l n) -> (v:a) -> Tot (seq1_st a n unit)
+let seq1_write #a #n i x = fun m ->  (), (m.[i] <- x)
+
+val seq1_bind: #a:Type -> #n:nat -> #b:Type -> #c:Type -> seq1_st a n b -> (b -> seq1_st a n c) -> Tot (seq1_st a n c)
+let seq1_bind #a #n #b #c f g = fun s -> let a, s = f s in g a s
+
+val seq1_iter: #a:Type -> #n:nat -> c:nat -> seq1_st a n unit -> Tot (seq1_st a n unit)
+let seq1_iter #a #m n f = 
+    let f' (s:seq_l a m) : Tot (seq_l a m) = 
+        let s' = f s in
+	snd s'
+    in
+    fun s -> (),iter 10 f' s
+
+val seq1_in_place_map2: #a:Type -> #n:nat -> #b:Type -> f:(a -> b -> Tot a) -> s:seq_l b n -> Tot (seq1_st a n unit)
+let seq1_in_place_map2  #a #m #b f i = 
+    fun s -> 
+      let s' = Spec.Loops.seq_map2 f s i in
+      (),s'
+
+val seq1_alloc: #a:Type -> #n:nat -> #b:Type -> init:a -> f:seq1_st a n b -> Tot b
+let seq1_alloc #a #n #b init f =
+    let s = Seq.create n init in
+    let s' = f s in
+    fst s'
+
+val seq1_uint32s_from_le: #n:nat -> b:bytes -> start:nat -> len: nat{
+						     length b = (4 ** len)
+					 	   /\ start + len <= n} -> 
+		     Tot (seq1_st u32 n unit) 
+let seq1_uint32s_from_le #n src start len =
+  fun s ->
+    let s' = uint32s_from_le len src in
+    let s0,s_ = split s start in
+    let s1,s2 = split s_ len in
+    (), s0 @| s' @| s2
+
+val seq1_uint32s_to_le: #n:nat -> start:nat -> len: nat{start + len <= n} -> 
+		     Tot (seq1_st u32 n (lbytes (4 ** len)))
+let seq1_uint32s_to_le #n start len =
+  fun s ->
+    if len = 0 then
+       Seq.createEmpty, s
+    else
+       let s0,s_ = split s start in
+       let s1,s2 = split s_ len in
+       let b = uint32s_to_le len s1 in
+       b, s
+
